\documentclass[aps,prd,preprint]{revtex4-1}
%\documentclass[aps,prd,final,twocolumn,floats,floatfix,nofootinbib,10pt]{revtex4-1}

% Note:  comment out one of the two documentclass commands, depending
% on whether you need the final or preprint version. It is most convenient
% to work in preprint mode, and switch to final only at the end.

\usepackage{graphicx}
\usepackage{amsmath}
\usepackage{amsfonts}
\usepackage{amssymb}
\usepackage{amstext}
\usepackage[english]{babel}
\usepackage{helvet}
\usepackage{microtype}
\usepackage{dsfont}
\usepackage[pdftex]{hyperref}
\usepackage{tikz}

\special{papersize=8.5in,11in}
\setlength{\pdfpageheight}{\paperheight}
\setlength{\pdfpagewidth}{\paperwidth}

\begin{document}

\title{2.21 in Baumgarte}
\author{indutny}
\date{\today}
\noaffiliation

\maketitle

\section{2.21}

\subsection{Problem statement}

Useful identities:
\begin{align}
\Omega_a = \nabla_a t, \\
\nabla_{[a} \Omega_{b]} = 0, \\
-\frac{1}{\alpha^2} = g^{ab} \Omega_a \Omega_b, \\
\omega_a = \alpha \Omega_a, \\
n^a = -g^{ab} \omega_b, \\
n^a n_a = -1, \\
\gamma^a_{\; b} = \delta^a_{\; b} + n^a n_b, \\
n^a \nabla_a n_b \equiv a_b, \\
\gamma^a_{\; b} \frac{\nabla_a \alpha}{\alpha} = a_b.
\end{align}

Prove that:
\begin{align}
{\cal{L}}_{\alpha n} \gamma^a_{\; b} = 0.
\end{align}

\subsection{Attempted solution}

\begin{align}
{\cal{L}}_{\alpha n} \gamma^a_{\; b} = &
  \alpha n^c \nabla_c \gamma^a_{\; b} +
  \nabla_b (\alpha n^c) \gamma^a_{\; c} -
  \nabla_c (\alpha n^a) \gamma^c_{\; b} \\
= & \alpha n^c \nabla_c (n^a n_b) +
  \underbrace{\gamma^a_{\; c} n^c}_{0}  \nabla_b \alpha + \alpha \gamma^a_{\; c} \nabla_b n^c -
  n^a \underbrace{\gamma^c_{\; b} \nabla_c \alpha}_{\alpha a_b} - \alpha \gamma^c_{\; b} \nabla_c n^a \\
= & \alpha n_b \underbrace{n^c \nabla_c n^a}_{a^a} + \alpha n^a \underbrace{n^c \nabla_c n_b}_{a_b} +
  \alpha \nabla_b n^a + \alpha n^a n_c \nabla_b n^c -   \alpha n^a a_b \\
& - \alpha \nabla_b n^a - \alpha n_b \underbrace{n^c \nabla_c n^a}_{a^a} \\
= & \alpha n^a n_c \nabla_b n^c = \alpha n^a \underbrace{ \nabla_b ( n_c n^c ) }_{0} - \alpha n^a n^c \nabla_b n_c \\
= & -n^a n^c \underbrace{\nabla_b (\alpha n_c)}_{-\nabla_b \omega_c} + n^a \underbrace{n^c n_c}_{-1} \nabla_b \alpha
\end{align}

\end{document}
